<rdf:RDF
    xmlns:rdf="http://www.w3.org/1999/02/22-rdf-syntax-ns#"
    xmlns:owl="http://www.w3.org/2002/07/owl#"
    xmlns:xsd="http://www.w3.org/2001/XMLSchema#"
    xmlns:rdfs="http://www.w3.org/2000/01/rdf-schema#" > 
  <rdf:Description rdf:about="http://purl.org/olia/olia.owl#PersReflPronoun">
    <rdf:type rdf:resource="http://www.w3.org/2002/07/owl#Class"/>
    <rdfs:subClassOf rdf:resource="http://purl.org/olia/olia.owl#Pronoun"/>
    <rdfs:comment>
			In Eagles personal and reflexive pronouns are brought together as a single value Pers./Refl. 		
			(http://www.ilc.cnr.it/EAGLES96/annotate/node17.html#recp 19.09.06)
		</rdfs:comment>
  </rdf:Description>
  <rdf:Description rdf:about="http://purl.org/olia/olia-top.owl#LinguisticConcept">
    <rdf:type rdf:resource="http://www.w3.org/2002/07/owl#Class"/>
    <rdfs:subClassOf rdf:resource="http://www.w3.org/2002/07/owl#Thing"/>
    <rdfs:comment>The OLiA ontology specifies linguistic concepts on a theoretical basis, as for concepts used in annotations, see system.owl.
There is a great extent of overlap between LinguisticCategories/LinguisticFeatures and Categories/Features as defined in system.owl.</rdfs:comment>
  </rdf:Description>
  <rdf:Description rdf:about="http://purl.org/olia/penn-syntax.owl#ExpletiveOfExtraposition">
    <rdf:type rdf:resource="http://www.w3.org/2002/07/owl#Class"/>
    <rdfs:comment>*EXP*
— Expletive (extraposition) ...
In cases where a clausal subject has been extraposed and replaced by an expletive it, we use a type of pseudo-attach called *EXP*. (In the small ATIS sample included with this release, it is also used for existential there.) Use of *EXP*-attach is discussed in more detail in section 17 [It-Extraposition]. 

  (S (NP-SBJ (NP It)
             (SBAR *EXP*-1))
     (VP is
         (ADJP-PRD clear)
         (PP to
             (NP me))
         (SBAR-1 that
                 (S (NP-SBJ this message)
                    (VP is
                        (ADJP-PRD unclear))))))

(Bies et al. 1995)</rdfs:comment>
    <rdfs:subClassOf rdf:resource="http://purl.org/olia/penn-syntax.owl#NullElement"/>
    <rdfs:subClassOf rdf:resource="http://purl.org/olia/olia.owl#ExpletivePronoun"/>
  </rdf:Description>
  <rdf:Description rdf:about="http://purl.org/olia/olia.owl#ExpletivePronoun">
    <rdf:type rdf:resource="http://www.w3.org/2002/07/owl#Class"/>
    <rdfs:subClassOf rdf:resource="http://purl.org/olia/olia.owl#ThirdPersonPronoun"/>
    <rdfs:subClassOf rdf:resource="http://purl.org/olia/olia.owl#Expletive"/>
    <rdfs:comment>
			An expletive (also known as a dummy word) is a part of speech whose members have no meaning, 
			but complete a sentence to make it grammatical [Crystal 1997, 127]
			(http://purl.org/linguistics/gold/Expletive)

			In European languages, expletives are pronouns. A verbal part of speech that 
			"has no meaning, but complete a sentence to make it grammatical" is a copula (see AuxiliaryVerb).
		</rdfs:comment>
  </rdf:Description>
  <rdf:Description rdf:about="http://purl.org/olia/olia.owl#Pronoun">
    <rdfs:comment>
		A pronoun is a pro-form which functions like a noun and substitutes for a 
		noun or a noun-phrase. A language may have several classes of pronouns.
		(http://www.sil.org/linguistics/GlossaryOfLinguisticTerms/WhatIsAPronoun.htm 19.09.06)
		
		A pronominal is a phrase that functions as a pronoun
        (www.sil.org/linguistics/GlossaryOfLinguisticTerms/WhatIsAPronominal.htm; http://www.isocat.org/datcat/DC-1369)
	</rdfs:comment>
    <rdfs:subClassOf rdf:resource="http://purl.org/olia/olia.owl#PronounOrDeterminer"/>
    <rdf:type rdf:resource="http://www.w3.org/2002/07/owl#Class"/>
  </rdf:Description>
  <rdf:Description rdf:about="http://purl.org/olia/olia-top.owl#SyntacticCategory">
    <rdf:type rdf:resource="http://www.w3.org/2002/07/owl#Class"/>
    <rdfs:subClassOf rdf:resource="http://purl.org/olia/olia-top.owl#LinguisticConcept"/>
  </rdf:Description>
  <rdf:Description rdf:about="http://purl.org/olia/system.owl#LinguisticAnnotation">
    <rdfs:comment>Linguistic annotations pertain to either structural entities (words, tokens, constituents, sentences =&gt; UnitOfAnnotation), relations between these (dependency, dominance, coreference, etc. =&gt; Relation), or grammatical features attached to these (case, gender, number, agreement, tense, mood, aspect, ... =&gt; Feature).</rdfs:comment>
    <rdfs:subClassOf rdf:resource="http://www.w3.org/2002/07/owl#Thing"/>
    <rdf:type rdf:resource="http://www.w3.org/2002/07/owl#Class"/>
  </rdf:Description>
  <rdf:Description rdf:about="http://purl.org/olia/olia-top.owl#MorphosyntacticCategory">
    <rdfs:subClassOf rdf:resource="http://purl.org/olia/olia-top.owl#SyntacticCategory"/>
    <rdf:type rdf:resource="http://www.w3.org/2002/07/owl#Class"/>
  </rdf:Description>
  <rdf:Description rdf:about="http://purl.org/olia/olia.owl#Expletive">
    <rdfs:label>expletive</rdfs:label>
    <rdfs:comment>
                            Word which serves no grammatical function, but which fills up a sentence or gives emphasis.
                                (www.southwestern.edu/~carlg/Latin_Web/glossary.html; http://www.isocat.org/datcat/DC-1283)
                            </rdfs:comment>
    <rdfs:subClassOf rdf:resource="http://purl.org/olia/olia.owl#Unique"/>
    <rdf:type rdf:resource="http://www.w3.org/2002/07/owl#Class"/>
  </rdf:Description>
  <rdf:Description rdf:about="http://purl.org/olia/olia-top.owl#Word">
    <rdfs:label>word</rdfs:label>
    <rdfs:comment>
		SyntacticWord is the class of syntactic units occupying the lowest position in 
		a syntactic construction. They are the largest units resistant to insertion of 
		new constituents within their boundaries; or they are the smallest constituents 
		that can be moved within a sentence without making the sentence ungrammatical.
		(http://www.linguistics-ontology.org/gold/2008/SyntacticWord)
		
		Linguistic unit composed of at least a part of speech and a lemma.
        (Gil Francopoulo; http://www.isocat.org/datcat/DC-1415)
	</rdfs:comment>
    <rdfs:subClassOf rdf:resource="http://purl.org/olia/olia-top.owl#SyntacticCategory"/>
    <rdf:type rdf:resource="http://www.w3.org/2002/07/owl#Class"/>
  </rdf:Description>
  <rdf:Description rdf:about="http://purl.org/olia/olia-top.owl#OrthographicEntity">
    <rdfs:subClassOf rdf:resource="http://purl.org/olia/olia-top.owl#LinguisticConcept"/>
    <rdf:type rdf:resource="http://www.w3.org/2002/07/owl#Class"/>
  </rdf:Description>
  <rdf:Description rdf:about="http://purl.org/olia/olia.owl#Token">
    <rdf:type rdf:resource="http://www.w3.org/2002/07/owl#Class"/>
    <rdfs:subClassOf rdf:resource="http://purl.org/olia/olia-top.owl#OrthographicEntity"/>
    <rdfs:comment>
                            Character string surrounded by separators.
                                (Gil Francopoulo; http://www.isocat.org/datcat/DC-1403)
                            </rdfs:comment>
    <rdfs:label>token</rdfs:label>
  </rdf:Description>
  <rdf:Description rdf:about="http://purl.org/olia/penn-syntax.owl#NullElement">
    <rdf:type rdf:resource="http://www.w3.org/2002/07/owl#Class"/>
    <rdfs:subClassOf rdf:resource="http://purl.org/olia/penn-syntax.owl#TokenLikeElement"/>
    <rdfs:comment>Modelled like tokens, Santorini (1991, §4.2), Bies (1995, §2.3, §2.5)</rdfs:comment>
  </rdf:Description>
  <rdf:Description rdf:about="http://www.w3.org/2002/07/owl#Thing">
    <rdf:type rdf:resource="http://www.w3.org/2002/07/owl#Class"/>
  </rdf:Description>
  <rdf:Description rdf:about="http://purl.org/olia/olia.owl#PronounOrDeterminer">
    <rdf:type rdf:resource="http://www.w3.org/2002/07/owl#Class"/>
    <rdfs:subClassOf rdf:resource="http://purl.org/olia/olia-top.owl#Word"/>
    <rdfs:subClassOf rdf:resource="http://purl.org/olia/olia-top.owl#MorphosyntacticCategory"/>
    <rdfs:comment>
		The parts of speech Pronoun, Determiner and Article heavily overlap in their formal and functional 
		characteristics, and different analyses for different languages entail separating them out in 
		different ways.
		In Eagles, Pronouns and Determiners are placed in one `super-category'. For some descriptions it may 
		be thought best to treat them as totally different parts of speech.
		(http://www.ilc.cnr.it/EAGLES96/annotate/node17.html#recp 19.09.06)
	</rdfs:comment>
  </rdf:Description>
  <rdf:Description rdf:about="http://purl.org/olia/system.owl#UnitOfAnnotation">
    <rdf:type rdf:resource="http://www.w3.org/2002/07/owl#Class"/>
    <rdfs:subClassOf rdf:resource="http://purl.org/olia/system.owl#LinguisticAnnotation"/>
    <rdfs:comment>A UnitOfAnnotation is a structural entity that can be annotated, e.g., a word, token, constituent, or another types of markable.
Word classes, etc., are then modelled as indirect children of UnitOfAnnotation. The division between Features and classes of UnitsOfAnnotation follows conventional standards.
    </rdfs:comment>
  </rdf:Description>
  <rdf:Description rdf:about="http://purl.org/olia/olia.owl#Unique">
    <rdf:type rdf:resource="http://www.w3.org/2002/07/owl#Class"/>
    <rdfs:subClassOf rdf:resource="http://purl.org/olia/olia-top.owl#Word"/>
    <rdfs:subClassOf rdf:resource="http://purl.org/olia/olia-top.owl#MorphosyntacticCategory"/>
    <rdfs:comment>
		Unique approximates the linguistic concept "Particle".
		It covers categories with unique or very small membership, 
		such as negative particle, which are `unassigned' to any of the standard part-of-speech categories. 
		(http://www.ilc.cnr.it/EAGLES96/annotate/node16.html#mp 19.09.06) 
	</rdfs:comment>
  </rdf:Description>
  <rdf:Description rdf:about="http://purl.org/olia/penn-syntax.owl#EXP">
    <rdf:type rdf:resource="http://www.w3.org/2002/07/owl#Thing"/>
  </rdf:Description>
  <rdf:Description rdf:about="http://purl.org/olia/olia.owl#ThirdPersonPronoun">
    <rdfs:comment>
			Third person reference is a deictic reference to a referent(s) not identified as the speaker or addressee.
			(http://www.sil.org/linguistics/GlossaryOfLinguisticTerms/WhatIsThirdPersonDeixis.htm 19.09.06)
		</rdfs:comment>
    <rdfs:subClassOf rdf:resource="http://purl.org/olia/olia.owl#PersReflPronoun"/>
    <rdf:type rdf:resource="http://www.w3.org/2002/07/owl#Class"/>
  </rdf:Description>
  <rdf:Description rdf:about="http://purl.org/olia/penn-syntax.owl#TokenLikeElement">
    <rdfs:comment>Special tokens and pseudo tokens for null elements.</rdfs:comment>
    <rdfs:subClassOf rdf:resource="http://purl.org/olia/system.owl#UnitOfAnnotation"/>
    <rdfs:subClassOf rdf:resource="http://purl.org/olia/olia.owl#Token"/>
    <rdf:type rdf:resource="http://www.w3.org/2002/07/owl#Class"/>
  </rdf:Description>
</rdf:RDF>
