<rdf:RDF
    xmlns:rdf="http://www.w3.org/1999/02/22-rdf-syntax-ns#"
    xmlns:owl="http://www.w3.org/2002/07/owl#"
    xmlns:xsd="http://www.w3.org/2001/XMLSchema#"
    xmlns:rdfs="http://www.w3.org/2000/01/rdf-schema#" > 
  <rdf:Description rdf:about="http://purl.org/olia/olia-top.owl#LinguisticConcept">
    <rdf:type rdf:resource="http://www.w3.org/2002/07/owl#Class"/>
    <rdfs:subClassOf rdf:resource="http://www.w3.org/2002/07/owl#Thing"/>
    <rdfs:comment>The OLiA ontology specifies linguistic concepts on a theoretical basis, as for concepts used in annotations, see system.owl.
There is a great extent of overlap between LinguisticCategories/LinguisticFeatures and Categories/Features as defined in system.owl.</rdfs:comment>
  </rdf:Description>
  <rdf:Description rdf:about="http://purl.org/olia/olia.owl#Modifier">
    <rdfs:comment>added in conformance with TIGER</rdfs:comment>
    <rdfs:subClassOf rdf:resource="http://purl.org/olia/olia-top.owl#SyntacticRole"/>
    <rdf:type rdf:resource="http://www.w3.org/2002/07/owl#Class"/>
  </rdf:Description>
  <rdf:Description rdf:about="http://purl.org/olia/penn-syntax.owl#MNR">
    <rdf:type rdf:resource="http://www.w3.org/2002/07/owl#Thing"/>
  </rdf:Description>
  <rdf:Description rdf:about="http://purl.org/olia/system.owl#LinguisticAnnotation">
    <rdfs:comment>Linguistic annotations pertain to either structural entities (words, tokens, constituents, sentences =&gt; UnitOfAnnotation), relations between these (dependency, dominance, coreference, etc. =&gt; Relation), or grammatical features attached to these (case, gender, number, agreement, tense, mood, aspect, ... =&gt; Feature).</rdfs:comment>
    <rdfs:subClassOf rdf:resource="http://www.w3.org/2002/07/owl#Thing"/>
    <rdf:type rdf:resource="http://www.w3.org/2002/07/owl#Class"/>
  </rdf:Description>
  <rdf:Description rdf:about="http://purl.org/olia/system.owl#Feature">
    <rdf:type rdf:resource="http://www.w3.org/2002/07/owl#Class"/>
    <rdfs:subClassOf rdf:resource="http://purl.org/olia/system.owl#LinguisticAnnotation"/>
    <rdfs:comment>UnitsOfAnnotation and Relations can be described in a more detailed way by the features that are attached to them, e.g., case, number, or aspect. Features are, however, not subject to further annotations (by means of hasFeature), they are thus disjoint from Relations and UnitsOfAnnotation.</rdfs:comment>
  </rdf:Description>
  <rdf:Description rdf:about="http://purl.org/olia/olia-top.owl#SemanticFeature">
    <rdf:type rdf:resource="http://www.w3.org/2002/07/owl#Class"/>
    <rdfs:subClassOf rdf:resource="http://purl.org/olia/system.owl#Feature"/>
    <rdfs:subClassOf rdf:resource="http://purl.org/olia/olia-top.owl#LinguisticConcept"/>
    <rdfs:comment></rdfs:comment>
  </rdf:Description>
  <rdf:Description rdf:about="http://purl.org/olia/olia.owl#SyntacticAdjunct">
    <rdfs:comment>
			Prototypically, an optional (morpho)syntactic constituent.

			'Satellites are not ... required by the predicate; they give 
			optional further information pertaining to additional features of the 
			SoA ..., the location of the SoA ..., the speaker's attitude towards 
			or evaluation of the propositional content ..., or the character of 
			the speech act...' (Dik, 1997:87)
			(http://languagelink.let.uu.nl/tds/onto/LinguisticOntology.owl#syntacticAdjunct)
			
			The category adjunct (ADJ) is assigned to those constituents that appear as optional additions, 
			be it to the main verb or to a given noun. This means that they can be left out freely without 
			a change in grammaticality or a significant change in meaning.
			In  "John called Mary (from school) (with his cell phone)"  the optional additions "from school" 
			and "with his cell phone" are such optional additions that can be left out freely.
			Adjuncts are generally used to convey additional information about the time, place, manner, or 
			cause of the event or situation described by the clause (see below). That is, they restrict the 
			class of events/  situations described by the clause to a subset. If required the category ADJ 
			can be split up into semantic sub-categories, that are annotated in layer semantic roles (time, 
			location, etc.).
			(Dipper et al. 2007, §4.3.3)
		</rdfs:comment>
    <rdfs:subClassOf rdf:resource="http://purl.org/olia/olia-top.owl#SyntacticRole"/>
    <rdf:type rdf:resource="http://www.w3.org/2002/07/owl#Class"/>
  </rdf:Description>
  <rdf:Description rdf:about="http://purl.org/olia/olia.owl#AdverbialModifier">
    <rdf:type rdf:resource="http://www.w3.org/2002/07/owl#Class"/>
    <rdfs:subClassOf rdf:resource="http://purl.org/olia/olia.owl#Modifier"/>
    <rdfs:subClassOf rdf:resource="http://purl.org/olia/olia.owl#SyntacticAdjunct"/>
    <rdfs:comment>
			An adverbial modifier modifies a verb.
			(http://languagelink.let.uu.nl/tds/onto/LinguisticOntology.owl#adverbialModifier)
		</rdfs:comment>
  </rdf:Description>
  <rdf:Description rdf:about="http://www.w3.org/2002/07/owl#Thing">
    <rdf:type rdf:resource="http://www.w3.org/2002/07/owl#Class"/>
  </rdf:Description>
  <rdf:Description rdf:about="http://purl.org/olia/penn-syntax.owl#FunctionTag">
    <rdfs:comment>Bies et al. (1995), func label of edges in TIGER</rdfs:comment>
    <rdfs:subClassOf rdf:resource="http://purl.org/olia/system.owl#Feature"/>
    <rdf:type rdf:resource="http://www.w3.org/2002/07/owl#Class"/>
  </rdf:Description>
  <rdf:Description rdf:about="http://purl.org/olia/olia-top.owl#SyntacticFeature">
    <rdfs:subClassOf rdf:resource="http://purl.org/olia/olia-top.owl#LinguisticConcept"/>
    <rdfs:subClassOf rdf:resource="http://purl.org/olia/system.owl#Feature"/>
    <rdf:type rdf:resource="http://www.w3.org/2002/07/owl#Class"/>
  </rdf:Description>
  <rdf:Description rdf:about="http://purl.org/olia/olia-top.owl#SyntacticRole">
    <rdf:type rdf:resource="http://www.w3.org/2002/07/owl#Class"/>
    <rdfs:subClassOf rdf:resource="http://purl.org/olia/olia-top.owl#SyntacticFeature"/>
    <rdfs:comment>Traditionally, "grammatical relations" or "grammatical roles" are specifically those between the verb (clause) and its arguments/adjunct/complementizer.
      In modern corpus research, however, a broad variety of relations between nominal heads, their arguments, modifiers, etc. are distinguished and the scope of "Grammatical Relation" has extended here to cover these as well.
      (http://purl.org/linguistics/gold/syntacticRole)</rdfs:comment>
  </rdf:Description>
  <rdf:Description rdf:about="http://purl.org/olia/penn-syntax.owl#Adjunct">
    <rdf:type rdf:resource="http://www.w3.org/2002/07/owl#Class"/>
    <rdfs:subClassOf rdf:resource="http://purl.org/olia/olia.owl#Modifier"/>
    <rdfs:subClassOf rdf:resource="http://purl.org/olia/penn-syntax.owl#FunctionTag"/>
    <rdfs:subClassOf rdf:resource="http://purl.org/olia/olia.owl#SyntacticAdjunct"/>
    <rdfs:comment>Adjuncts are also represented as sisters of heads. 
Let’s (VP meet (PP on Tuesday))
(Santorini 1991)

cf. Adverbials (Bies et al. 1995, § 2.2.3)</rdfs:comment>
  </rdf:Description>
  <rdf:Description rdf:about="http://purl.org/olia/olia.owl#MannerRole">
    <rdf:type rdf:resource="http://www.w3.org/2002/07/owl#Class"/>
    <rdfs:subClassOf rdf:resource="http://purl.org/olia/olia-top.owl#SemanticRole"/>
    <rdfs:comment>
			Manner applies to constituents that denote how something is carried out.
			Adverbs may also denote manner, however, they are not annotated at any of the
			syntactic layers.
			(Dipper et al. 2007, §5.3.11)
		</rdfs:comment>
  </rdf:Description>
  <rdf:Description rdf:about="http://purl.org/olia/penn-syntax.owl#MannerAdverbial">
    <rdf:type rdf:resource="http://www.w3.org/2002/07/owl#Class"/>
    <rdfs:comment>-MNR (manner)
— marks adverbials that indicate manner, including instrument phrases. 

  (S (NP She)
     (VP waited
         (ADVP-MNR impatiently)))
(Bies et al. 1995)</rdfs:comment>
    <rdfs:subClassOf rdf:resource="http://purl.org/olia/olia.owl#AdverbialModifier"/>
    <rdfs:subClassOf rdf:resource="http://purl.org/olia/penn-syntax.owl#Adjunct"/>
    <rdfs:subClassOf rdf:resource="http://purl.org/olia/olia.owl#MannerRole"/>
  </rdf:Description>
  <rdf:Description rdf:about="http://purl.org/olia/olia-top.owl#SemanticRole">
    <rdfs:comment>
        In linguistics, a theta role or θ-role is the semantic role a noun 
        phrase plays in a sentence. The term Thematic role denotes the same 
        concept. As such it is a semantic rather than a syntactic feature, in 
        contrast to such notions as the subject of a sentence or a 
        prepositional object. 
        (http://en.wikipedia.org/wiki/Subject_(linguistics).
		
		Originally, semantic roles were referred to as "case roles", leading to
		an unfortunate name clash with grammatical case (e.g. in GOLD CaseValue)
	</rdfs:comment>
    <rdfs:subClassOf rdf:resource="http://purl.org/olia/olia-top.owl#SemanticFeature"/>
    <rdf:type rdf:resource="http://www.w3.org/2002/07/owl#Class"/>
  </rdf:Description>
</rdf:RDF>
