@prefix rdfs:    <http://www.w3.org/2000/01/rdf-schema#> .
@prefix owl:     <http://www.w3.org/2002/07/owl#> .
@prefix xsd:     <http://www.w3.org/2001/XMLSchema#> .
@prefix rdf:     <http://www.w3.org/1999/02/22-rdf-syntax-ns#> .

<http://purl.org/olia/penn.owl#CoordinatingConjunction>
      a       owl:Class ;
      rdfs:comment """This category includes \"and\", \"but\", \"nor\", \"or\", \"yet\" (as in \"Yet it's cheap\", \"cheap yet good\"), as well as the mathematical operators \"plus\", \"minus\", \"less\", \"times\" (in the sense of \"multiplied by\") and \"over\" (in the sense of \"divided by\"), when they are spelled out.
For in the sense of \"because\" is a coordinating conjunction.""" ;
      rdfs:subClassOf <http://purl.org/olia/olia.owl#CoordinatingConjunction> , <http://purl.org/olia/penn.owl#Conjunction> .

<http://purl.org/olia/olia.owl#CoordinatingConjunction>
      a       owl:Class ;
      rdfs:comment """
			Coordinating conjunctions, also called coordinators, are conjunctions that 
			join two items of equal syntactic importance.
			(http://en.wikipedia.org/wiki/Grammatical_conjunction 19.09.06)
		""" ;
      rdfs:subClassOf <http://purl.org/olia/olia.owl#Conjunction> .

<http://purl.org/olia/olia.owl#Conjunction>
      a       owl:Class ;
      rdfs:comment """
		A conjunction is a word that syntactically links words or larger constituents, 
		and expresses a semantic relationship between them.
		(http://www.sil.org/linguistics/GlossaryOfLinguisticTerms/WhatIsAConjunction.htm 19.09.06)
	""" ;
      rdfs:subClassOf <http://purl.org/olia/olia-top.owl#MorphosyntacticCategory> , <http://purl.org/olia/olia-top.owl#Word> .

owl:Thing
      a       owl:Class .

<http://purl.org/olia/olia-top.owl#LinguisticConcept>
      a       owl:Class ;
      rdfs:comment """The OLiA ontology specifies linguistic concepts on a theoretical basis, as for concepts used in annotations, see system.owl.
There is a great extent of overlap between LinguisticCategories/LinguisticFeatures and Categories/Features as defined in system.owl.""" ;
      rdfs:subClassOf owl:Thing .

<http://purl.org/olia/penn.owl#Tag>
      a       owl:Class ;
      rdfs:subClassOf <http://purl.org/olia/system.owl#LinguisticAnnotation> .

<http://purl.org/olia/system.owl#LinguisticAnnotation>
      a       owl:Class ;
      rdfs:comment "Linguistic annotations pertain to either structural entities (words, tokens, constituents, sentences => UnitOfAnnotation), relations between these (dependency, dominance, coreference, etc. => Relation), or grammatical features attached to these (case, gender, number, agreement, tense, mood, aspect, ... => Feature)." ;
      rdfs:subClassOf owl:Thing .

<http://purl.org/olia/olia-top.owl#MorphosyntacticCategory>
      a       owl:Class ;
      rdfs:subClassOf <http://purl.org/olia/olia-top.owl#SyntacticCategory> .

<http://purl.org/olia/olia-top.owl#SyntacticCategory>
      a       owl:Class ;
      rdfs:subClassOf <http://purl.org/olia/olia-top.owl#LinguisticConcept> .

<http://purl.org/olia/penn.owl#CC>
      a       owl:Thing .

<http://purl.org/olia/olia-top.owl#Word>
      a       owl:Class ;
      rdfs:comment """
		SyntacticWord is the class of syntactic units occupying the lowest position in 
		a syntactic construction. They are the largest units resistant to insertion of 
		new constituents within their boundaries; or they are the smallest constituents 
		that can be moved within a sentence without making the sentence ungrammatical.
		(http://www.linguistics-ontology.org/gold/2008/SyntacticWord)
		
		Linguistic unit composed of at least a part of speech and a lemma.
        (Gil Francopoulo; http://www.isocat.org/datcat/DC-1415)
	""" ;
      rdfs:label "word" ;
      rdfs:subClassOf <http://purl.org/olia/olia-top.owl#SyntacticCategory> .

<http://purl.org/olia/penn.owl#Conjunction>
      a       owl:Class ;
      rdfs:comment """This class was inserted to reflect the tag structure. It does not, 
    however, exactly correspond to olia:Conjunction, because Penn conjunction 
    tags can also be applied to prepositions.""" ;
      rdfs:subClassOf <http://purl.org/olia/penn.owl#Tag> .
