@prefix rdfs:    <http://www.w3.org/2000/01/rdf-schema#> .
@prefix owl:     <http://www.w3.org/2002/07/owl#> .
@prefix xsd:     <http://www.w3.org/2001/XMLSchema#> .
@prefix rdf:     <http://www.w3.org/1999/02/22-rdf-syntax-ns#> .

<http://purl.org/olia/olia-top.owl#LinguisticConcept>
      a       owl:Class ;
      rdfs:comment """The OLiA ontology specifies linguistic concepts on a theoretical basis, as for concepts used in annotations, see system.owl.
There is a great extent of overlap between LinguisticCategories/LinguisticFeatures and Categories/Features as defined in system.owl.""" ;
      rdfs:subClassOf owl:Thing .

<http://purl.org/olia/olia.owl#Comparative>
      a       owl:Class ;
      rdfs:comment """
			The comparative is the form of an adjective or adverb which denotes 
			the degree or grade by which a person, thing, or other entity has a 
			property or quality greater or less in extent than that of another. 
			In English the structure of a comparative consists normally of the 
			positive form of the adjective or adverb, plus the suffix -er, or 
			(especially in the case of longer words) the modifier \"more\" (or 
			\"less\") before the adjective or adverb. The form is usually completed 
			by \"than\" and the noun which is being compared, e.g. \"he is taller 
			than his father is\", or \"the village is less picturesque than the 
			town near by is\". (http://en.wikipedia.org/wiki/Comparative  17.11.06)
		""" ;
      rdfs:subClassOf <http://purl.org/olia/olia-top.owl#DegreeFeature> .

<http://purl.org/olia/olia-top.owl#SyntacticCategory>
      a       owl:Class ;
      rdfs:subClassOf <http://purl.org/olia/olia-top.owl#LinguisticConcept> .

<http://purl.org/olia/system.owl#LinguisticAnnotation>
      a       owl:Class ;
      rdfs:comment "Linguistic annotations pertain to either structural entities (words, tokens, constituents, sentences => UnitOfAnnotation), relations between these (dependency, dominance, coreference, etc. => Relation), or grammatical features attached to these (case, gender, number, agreement, tense, mood, aspect, ... => Feature)." ;
      rdfs:subClassOf owl:Thing .

<http://purl.org/olia/olia-top.owl#MorphosyntacticCategory>
      a       owl:Class ;
      rdfs:subClassOf <http://purl.org/olia/olia-top.owl#SyntacticCategory> .

<http://purl.org/olia/olia.owl#Adjective>
      a       owl:Class ;
      rdfs:comment """
		An Adjective is a noun-modifying expression that specifies the properties or attributes of the nominal referent.
		(http://www.sil.org/linguistics/GlossaryOfLinguisticTerms/WhatIsAnAdjective.htm  18.9.06)
	""" ;
      rdfs:subClassOf <http://purl.org/olia/olia-top.owl#MorphosyntacticCategory> , <http://purl.org/olia/olia-top.owl#Word> .

<http://purl.org/olia/olia-top.owl#DegreeFeature>
      a       owl:Class ;
      rdfs:comment "The Eagles-recommended attribute Degree applies only to inflectional comparatives and superlatives. In some languages, e.g. Spanish, the number of such adjectives is very small. (http://www.ilc.cnr.it/EAGLES96/annotate/node17.html#recn)" ;
      rdfs:subClassOf <http://purl.org/olia/olia-top.owl#MorphosyntacticFeature> .

<http://purl.org/olia/olia-top.owl#MorphosyntacticFeature>
      a       owl:Class ;
      rdfs:comment "Morphosyntactic and morphological features." ;
      rdfs:subClassOf <http://purl.org/olia/olia-top.owl#LinguisticConcept> , <http://purl.org/olia/system.owl#Feature> .

<http://purl.org/olia/olia-top.owl#Word>
      a       owl:Class ;
      rdfs:comment """
		SyntacticWord is the class of syntactic units occupying the lowest position in 
		a syntactic construction. They are the largest units resistant to insertion of 
		new constituents within their boundaries; or they are the smallest constituents 
		that can be moved within a sentence without making the sentence ungrammatical.
		(http://www.linguistics-ontology.org/gold/2008/SyntacticWord)
		
		Linguistic unit composed of at least a part of speech and a lemma.
        (Gil Francopoulo; http://www.isocat.org/datcat/DC-1415)
	""" ;
      rdfs:label "word" ;
      rdfs:subClassOf <http://purl.org/olia/olia-top.owl#SyntacticCategory> .

<http://purl.org/olia/penn.owl#JJR>
      a       owl:Thing .

<http://purl.org/olia/system.owl#Feature>
      a       owl:Class ;
      rdfs:comment "UnitsOfAnnotation and Relations can be described in a more detailed way by the features that are attached to them, e.g., case, number, or aspect. Features are, however, not subject to further annotations (by means of hasFeature), they are thus disjoint from Relations and UnitsOfAnnotation." ;
      rdfs:subClassOf <http://purl.org/olia/system.owl#LinguisticAnnotation> .

owl:Thing
      a       owl:Class .

<http://purl.org/olia/penn.owl#Tag>
      a       owl:Class ;
      rdfs:subClassOf <http://purl.org/olia/system.owl#LinguisticAnnotation> .

<http://purl.org/olia/penn.owl#ComparativeAdjective>
      a       owl:Class ;
      rdfs:comment """These are adjectives mostly with the comparative ending -er and a comparative meaning. \"More\" or \"less\" should be tagged as a comparative adjective when it is used without a head noun and it
corresponds to the object of a verb or preposition.""" ;
      rdfs:subClassOf <http://purl.org/olia/olia.owl#Comparative> , <http://purl.org/olia/penn.owl#Adjective> .

<http://purl.org/olia/penn.owl#Adjective>
      a       owl:Class ;
      rdfs:comment """These are adjectives, ordinal numerals, and ordinal numbers.
Hyphenated compounds that are used as modifiers are tagged as adjectives, e.g. \"happy-go-lucky\", \"one-of-a-kind\", \"run-of-the-mill\". Ordinal numbers are tagged as adjectives, as are compounds of the form \"n-th\" or \"X-est\", like \"fourth-largest\".""" ;
      rdfs:subClassOf <http://purl.org/olia/penn.owl#Tag> , <http://purl.org/olia/olia.owl#Adjective> .
