<rdf:RDF
    xmlns:rdf="http://www.w3.org/1999/02/22-rdf-syntax-ns#"
    xmlns:owl="http://www.w3.org/2002/07/owl#"
    xmlns:xsd="http://www.w3.org/2001/XMLSchema#"
    xmlns:rdfs="http://www.w3.org/2000/01/rdf-schema#" > 
  <rdf:Description rdf:about="http://purl.org/olia/olia-top.owl#LinguisticConcept">
    <rdfs:comment>The OLiA ontology specifies linguistic concepts on a theoretical basis, as for concepts used in annotations, see system.owl.
There is a great extent of overlap between LinguisticCategories/LinguisticFeatures and Categories/Features as defined in system.owl.</rdfs:comment>
    <rdfs:subClassOf rdf:resource="http://www.w3.org/2002/07/owl#Thing"/>
    <rdf:type rdf:resource="http://www.w3.org/2002/07/owl#Class"/>
  </rdf:Description>
  <rdf:Description rdf:about="http://purl.org/olia/olia.owl#Superlative">
    <rdf:type rdf:resource="http://www.w3.org/2002/07/owl#Class"/>
    <rdfs:subClassOf rdf:resource="http://purl.org/olia/olia-top.owl#DegreeFeature"/>
    <rdfs:comment>
			The superlative of an adjective or adverb is a form of adjective or 
			adverb which indicates that something has some feature to a greater 
			degree than anything it is being compared to in a given context. 
			(http://en.wikipedia.org/wiki/Superlative  17.11.06)
		</rdfs:comment>
  </rdf:Description>
  <rdf:Description rdf:about="http://purl.org/olia/penn.owl#JJS">
    <rdf:type rdf:resource="http://www.w3.org/2002/07/owl#Thing"/>
  </rdf:Description>
  <rdf:Description rdf:about="http://purl.org/olia/olia-top.owl#SyntacticCategory">
    <rdfs:subClassOf rdf:resource="http://purl.org/olia/olia-top.owl#LinguisticConcept"/>
    <rdf:type rdf:resource="http://www.w3.org/2002/07/owl#Class"/>
  </rdf:Description>
  <rdf:Description rdf:about="http://purl.org/olia/system.owl#LinguisticAnnotation">
    <rdf:type rdf:resource="http://www.w3.org/2002/07/owl#Class"/>
    <rdfs:subClassOf rdf:resource="http://www.w3.org/2002/07/owl#Thing"/>
    <rdfs:comment>Linguistic annotations pertain to either structural entities (words, tokens, constituents, sentences =&gt; UnitOfAnnotation), relations between these (dependency, dominance, coreference, etc. =&gt; Relation), or grammatical features attached to these (case, gender, number, agreement, tense, mood, aspect, ... =&gt; Feature).</rdfs:comment>
  </rdf:Description>
  <rdf:Description rdf:about="http://purl.org/olia/olia-top.owl#MorphosyntacticCategory">
    <rdf:type rdf:resource="http://www.w3.org/2002/07/owl#Class"/>
    <rdfs:subClassOf rdf:resource="http://purl.org/olia/olia-top.owl#SyntacticCategory"/>
  </rdf:Description>
  <rdf:Description rdf:about="http://purl.org/olia/olia.owl#Adjective">
    <rdfs:comment>
		An Adjective is a noun-modifying expression that specifies the properties or attributes of the nominal referent.
		(http://www.sil.org/linguistics/GlossaryOfLinguisticTerms/WhatIsAnAdjective.htm  18.9.06)
	</rdfs:comment>
    <rdfs:subClassOf rdf:resource="http://purl.org/olia/olia-top.owl#MorphosyntacticCategory"/>
    <rdfs:subClassOf rdf:resource="http://purl.org/olia/olia-top.owl#Word"/>
    <rdf:type rdf:resource="http://www.w3.org/2002/07/owl#Class"/>
  </rdf:Description>
  <rdf:Description rdf:about="http://purl.org/olia/olia-top.owl#DegreeFeature">
    <rdfs:comment>The Eagles-recommended attribute Degree applies only to inflectional comparatives and superlatives. In some languages, e.g. Spanish, the number of such adjectives is very small. (http://www.ilc.cnr.it/EAGLES96/annotate/node17.html#recn)</rdfs:comment>
    <rdfs:subClassOf rdf:resource="http://purl.org/olia/olia-top.owl#MorphosyntacticFeature"/>
    <rdf:type rdf:resource="http://www.w3.org/2002/07/owl#Class"/>
  </rdf:Description>
  <rdf:Description rdf:about="http://purl.org/olia/olia-top.owl#MorphosyntacticFeature">
    <rdf:type rdf:resource="http://www.w3.org/2002/07/owl#Class"/>
    <rdfs:subClassOf rdf:resource="http://purl.org/olia/system.owl#Feature"/>
    <rdfs:subClassOf rdf:resource="http://purl.org/olia/olia-top.owl#LinguisticConcept"/>
    <rdfs:comment>Morphosyntactic and morphological features.</rdfs:comment>
  </rdf:Description>
  <rdf:Description rdf:about="http://purl.org/olia/olia-top.owl#Word">
    <rdf:type rdf:resource="http://www.w3.org/2002/07/owl#Class"/>
    <rdfs:subClassOf rdf:resource="http://purl.org/olia/olia-top.owl#SyntacticCategory"/>
    <rdfs:comment>
		SyntacticWord is the class of syntactic units occupying the lowest position in 
		a syntactic construction. They are the largest units resistant to insertion of 
		new constituents within their boundaries; or they are the smallest constituents 
		that can be moved within a sentence without making the sentence ungrammatical.
		(http://www.linguistics-ontology.org/gold/2008/SyntacticWord)
		
		Linguistic unit composed of at least a part of speech and a lemma.
        (Gil Francopoulo; http://www.isocat.org/datcat/DC-1415)
	</rdfs:comment>
    <rdfs:label>word</rdfs:label>
  </rdf:Description>
  <rdf:Description rdf:about="http://purl.org/olia/system.owl#Feature">
    <rdfs:comment>UnitsOfAnnotation and Relations can be described in a more detailed way by the features that are attached to them, e.g., case, number, or aspect. Features are, however, not subject to further annotations (by means of hasFeature), they are thus disjoint from Relations and UnitsOfAnnotation.</rdfs:comment>
    <rdfs:subClassOf rdf:resource="http://purl.org/olia/system.owl#LinguisticAnnotation"/>
    <rdf:type rdf:resource="http://www.w3.org/2002/07/owl#Class"/>
  </rdf:Description>
  <rdf:Description rdf:about="http://www.w3.org/2002/07/owl#Thing">
    <rdf:type rdf:resource="http://www.w3.org/2002/07/owl#Class"/>
  </rdf:Description>
  <rdf:Description rdf:about="http://purl.org/olia/penn.owl#SuperlativeAdjective">
    <rdf:type rdf:resource="http://www.w3.org/2002/07/owl#Class"/>
    <rdfs:comment>These are adjectives with the superlative ending -est (as well as "worst"). "Most" and "least" can also be tagged as superlative adjective when they occur by themselves.</rdfs:comment>
    <rdfs:subClassOf rdf:resource="http://purl.org/olia/olia.owl#Superlative"/>
    <rdfs:subClassOf rdf:resource="http://purl.org/olia/penn.owl#Adjective"/>
  </rdf:Description>
  <rdf:Description rdf:about="http://purl.org/olia/penn.owl#Tag">
    <rdfs:subClassOf rdf:resource="http://purl.org/olia/system.owl#LinguisticAnnotation"/>
    <rdf:type rdf:resource="http://www.w3.org/2002/07/owl#Class"/>
  </rdf:Description>
  <rdf:Description rdf:about="http://purl.org/olia/penn.owl#Adjective">
    <rdf:type rdf:resource="http://www.w3.org/2002/07/owl#Class"/>
    <rdfs:subClassOf rdf:resource="http://purl.org/olia/olia.owl#Adjective"/>
    <rdfs:subClassOf rdf:resource="http://purl.org/olia/penn.owl#Tag"/>
    <rdfs:comment>These are adjectives, ordinal numerals, and ordinal numbers.
Hyphenated compounds that are used as modifiers are tagged as adjectives, e.g. "happy-go-lucky", "one-of-a-kind", "run-of-the-mill". Ordinal numbers are tagged as adjectives, as are compounds of the form "n-th" or "X-est", like "fourth-largest".</rdfs:comment>
  </rdf:Description>
</rdf:RDF>
