<rdf:RDF
    xmlns:rdf="http://www.w3.org/1999/02/22-rdf-syntax-ns#"
    xmlns:owl="http://www.w3.org/2002/07/owl#"
    xmlns:xsd="http://www.w3.org/2001/XMLSchema#"
    xmlns:rdfs="http://www.w3.org/2000/01/rdf-schema#" > 
  <rdf:Description rdf:about="http://purl.org/olia/olia-top.owl#NumberFeature">
    <rdf:type rdf:resource="http://www.w3.org/2002/07/owl#Class"/>
    <rdfs:subClassOf rdf:resource="http://purl.org/olia/olia-top.owl#MorphosyntacticFeature"/>
    <rdfs:comment>
            Grammatical category for the variation in form of nouns, pronouns, and any words agreeing 
			with them, depending on how many persons or things are referred to.
            (www.wordreference.com/English/definition.asp?en=number 12; http://www.isocat.org/datcat/DC-1298)

			A grammatical number is a morphological category characterized by the expression of quantity 
			through inflection or agreement. (http://en.wikipedia.org/wiki/Grammatical_number  17.11.06)</rdfs:comment>
  </rdf:Description>
  <rdf:Description rdf:about="http://purl.org/olia/olia-top.owl#LinguisticConcept">
    <rdf:type rdf:resource="http://www.w3.org/2002/07/owl#Class"/>
    <rdfs:subClassOf rdf:resource="http://www.w3.org/2002/07/owl#Thing"/>
    <rdfs:comment>The OLiA ontology specifies linguistic concepts on a theoretical basis, as for concepts used in annotations, see system.owl.
There is a great extent of overlap between LinguisticCategories/LinguisticFeatures and Categories/Features as defined in system.owl.</rdfs:comment>
  </rdf:Description>
  <rdf:Description rdf:about="http://purl.org/olia/olia-top.owl#SyntacticCategory">
    <rdfs:subClassOf rdf:resource="http://purl.org/olia/olia-top.owl#LinguisticConcept"/>
    <rdf:type rdf:resource="http://www.w3.org/2002/07/owl#Class"/>
  </rdf:Description>
  <rdf:Description rdf:about="http://purl.org/olia/system.owl#LinguisticAnnotation">
    <rdf:type rdf:resource="http://www.w3.org/2002/07/owl#Class"/>
    <rdfs:subClassOf rdf:resource="http://www.w3.org/2002/07/owl#Thing"/>
    <rdfs:comment>Linguistic annotations pertain to either structural entities (words, tokens, constituents, sentences =&gt; UnitOfAnnotation), relations between these (dependency, dominance, coreference, etc. =&gt; Relation), or grammatical features attached to these (case, gender, number, agreement, tense, mood, aspect, ... =&gt; Feature).</rdfs:comment>
  </rdf:Description>
  <rdf:Description rdf:about="http://purl.org/olia/olia-top.owl#MorphosyntacticCategory">
    <rdf:type rdf:resource="http://www.w3.org/2002/07/owl#Class"/>
    <rdfs:subClassOf rdf:resource="http://purl.org/olia/olia-top.owl#SyntacticCategory"/>
  </rdf:Description>
  <rdf:Description rdf:about="http://purl.org/olia/olia-top.owl#MorphosyntacticFeature">
    <rdfs:comment>Morphosyntactic and morphological features.</rdfs:comment>
    <rdfs:subClassOf rdf:resource="http://purl.org/olia/olia-top.owl#LinguisticConcept"/>
    <rdfs:subClassOf rdf:resource="http://purl.org/olia/system.owl#Feature"/>
    <rdf:type rdf:resource="http://www.w3.org/2002/07/owl#Class"/>
  </rdf:Description>
  <rdf:Description rdf:about="http://purl.org/olia/olia-top.owl#Word">
    <rdf:type rdf:resource="http://www.w3.org/2002/07/owl#Class"/>
    <rdfs:subClassOf rdf:resource="http://purl.org/olia/olia-top.owl#SyntacticCategory"/>
    <rdfs:comment>
		SyntacticWord is the class of syntactic units occupying the lowest position in 
		a syntactic construction. They are the largest units resistant to insertion of 
		new constituents within their boundaries; or they are the smallest constituents 
		that can be moved within a sentence without making the sentence ungrammatical.
		(http://www.linguistics-ontology.org/gold/2008/SyntacticWord)
		
		Linguistic unit composed of at least a part of speech and a lemma.
        (Gil Francopoulo; http://www.isocat.org/datcat/DC-1415)
	</rdfs:comment>
    <rdfs:label>word</rdfs:label>
  </rdf:Description>
  <rdf:Description rdf:about="http://purl.org/olia/system.owl#Feature">
    <rdf:type rdf:resource="http://www.w3.org/2002/07/owl#Class"/>
    <rdfs:subClassOf rdf:resource="http://purl.org/olia/system.owl#LinguisticAnnotation"/>
    <rdfs:comment>UnitsOfAnnotation and Relations can be described in a more detailed way by the features that are attached to them, e.g., case, number, or aspect. Features are, however, not subject to further annotations (by means of hasFeature), they are thus disjoint from Relations and UnitsOfAnnotation.</rdfs:comment>
  </rdf:Description>
  <rdf:Description rdf:about="http://purl.org/olia/penn.owl#ProperNoun">
    <rdf:type rdf:resource="http://www.w3.org/2002/07/owl#Class"/>
    <rdfs:comment>These are singular or plural proper nouns.</rdfs:comment>
    <rdfs:subClassOf rdf:resource="http://purl.org/olia/penn.owl#Noun"/>
    <rdfs:subClassOf rdf:resource="http://purl.org/olia/olia.owl#ProperNoun"/>
  </rdf:Description>
  <rdf:Description rdf:about="http://purl.org/olia/olia.owl#Noun">
    <rdfs:comment>
	A noun, or noun substantive, is a part of speech (a word or phrase) which can co-occur with 
	(in)definite articles and attributive adjectives, and function as the head of a noun phrase.

	The word "noun" derives from the Latin 'nomen' meaning "name", and a traditional definition 
	of nouns is that they are all and only those expressions that refer to a person, place, 
	thing, event, substance, quality, idea or an appointment. They serve as the subject or object 
	of a verb, and the object of a preposition.
	(http://en.wikipedia.org/wiki/Noun 19.09.06)
	</rdfs:comment>
    <rdfs:subClassOf rdf:resource="http://purl.org/olia/olia-top.owl#MorphosyntacticCategory"/>
    <rdfs:subClassOf rdf:resource="http://purl.org/olia/olia-top.owl#Word"/>
    <rdf:type rdf:resource="http://www.w3.org/2002/07/owl#Class"/>
  </rdf:Description>
  <rdf:Description rdf:about="http://purl.org/olia/penn.owl#NNP">
    <rdf:type rdf:resource="http://www.w3.org/2002/07/owl#Thing"/>
  </rdf:Description>
  <rdf:Description rdf:about="http://purl.org/olia/olia.owl#Singular">
    <rdf:type rdf:resource="http://www.w3.org/2002/07/owl#Class"/>
    <rdfs:comment>
			Singular is a grammatical number denoting a unit quantity (as opposed 
			to the plural and other forms). (http://en.wikipedia.org/wiki/Singular
			17.11.06)
		</rdfs:comment>
    <rdfs:subClassOf rdf:resource="http://purl.org/olia/olia-top.owl#NumberFeature"/>
  </rdf:Description>
  <rdf:Description rdf:about="http://purl.org/olia/penn.owl#Noun">
    <rdf:type rdf:resource="http://www.w3.org/2002/07/owl#Class"/>
    <rdfs:subClassOf rdf:resource="http://purl.org/olia/penn.owl#Tag"/>
    <rdfs:subClassOf rdf:resource="http://purl.org/olia/olia.owl#Noun"/>
    <rdfs:comment>We inserted this class 'noun' to get a clearer ontology structure. In The Penn Treebank Tag Set there is no class 'noun'.</rdfs:comment>
  </rdf:Description>
  <rdf:Description rdf:about="http://www.w3.org/2002/07/owl#Thing">
    <rdf:type rdf:resource="http://www.w3.org/2002/07/owl#Class"/>
  </rdf:Description>
  <rdf:Description rdf:about="http://purl.org/olia/penn.owl#Tag">
    <rdfs:subClassOf rdf:resource="http://purl.org/olia/system.owl#LinguisticAnnotation"/>
    <rdf:type rdf:resource="http://www.w3.org/2002/07/owl#Class"/>
  </rdf:Description>
  <rdf:Description rdf:about="http://purl.org/olia/olia.owl#ProperNoun">
    <rdf:type rdf:resource="http://www.w3.org/2002/07/owl#Class"/>
    <rdfs:subClassOf rdf:resource="http://purl.org/olia/olia.owl#Noun"/>
    <rdfs:comment>
		Proper nouns (also called proper names) are the names of unique entities. 
		(http://en.wikipedia.org/wiki/Noun 19.09.06)
	</rdfs:comment>
  </rdf:Description>
</rdf:RDF>
