@prefix rdfs:    <http://www.w3.org/2000/01/rdf-schema#> .
@prefix owl:     <http://www.w3.org/2002/07/owl#> .
@prefix xsd:     <http://www.w3.org/2001/XMLSchema#> .
@prefix rdf:     <http://www.w3.org/1999/02/22-rdf-syntax-ns#> .

<http://purl.org/olia/olia-top.owl#NumberFeature>
      a       owl:Class ;
      rdfs:comment """
            Grammatical category for the variation in form of nouns, pronouns, and any words agreeing 
			with them, depending on how many persons or things are referred to.
            (www.wordreference.com/English/definition.asp?en=number 12; http://www.isocat.org/datcat/DC-1298)

			A grammatical number is a morphological category characterized by the expression of quantity 
			through inflection or agreement. (http://en.wikipedia.org/wiki/Grammatical_number  17.11.06)""" ;
      rdfs:subClassOf <http://purl.org/olia/olia-top.owl#MorphosyntacticFeature> .

<http://purl.org/olia/olia-top.owl#LinguisticConcept>
      a       owl:Class ;
      rdfs:comment """The OLiA ontology specifies linguistic concepts on a theoretical basis, as for concepts used in annotations, see system.owl.
There is a great extent of overlap between LinguisticCategories/LinguisticFeatures and Categories/Features as defined in system.owl.""" ;
      rdfs:subClassOf owl:Thing .

<http://purl.org/olia/olia-top.owl#SyntacticCategory>
      a       owl:Class ;
      rdfs:subClassOf <http://purl.org/olia/olia-top.owl#LinguisticConcept> .

<http://purl.org/olia/system.owl#LinguisticAnnotation>
      a       owl:Class ;
      rdfs:comment "Linguistic annotations pertain to either structural entities (words, tokens, constituents, sentences => UnitOfAnnotation), relations between these (dependency, dominance, coreference, etc. => Relation), or grammatical features attached to these (case, gender, number, agreement, tense, mood, aspect, ... => Feature)." ;
      rdfs:subClassOf owl:Thing .

<http://purl.org/olia/olia-top.owl#MorphosyntacticCategory>
      a       owl:Class ;
      rdfs:subClassOf <http://purl.org/olia/olia-top.owl#SyntacticCategory> .

<http://purl.org/olia/olia-top.owl#MorphosyntacticFeature>
      a       owl:Class ;
      rdfs:comment "Morphosyntactic and morphological features." ;
      rdfs:subClassOf <http://purl.org/olia/olia-top.owl#LinguisticConcept> , <http://purl.org/olia/system.owl#Feature> .

<http://purl.org/olia/olia-top.owl#Word>
      a       owl:Class ;
      rdfs:comment """
		SyntacticWord is the class of syntactic units occupying the lowest position in 
		a syntactic construction. They are the largest units resistant to insertion of 
		new constituents within their boundaries; or they are the smallest constituents 
		that can be moved within a sentence without making the sentence ungrammatical.
		(http://www.linguistics-ontology.org/gold/2008/SyntacticWord)
		
		Linguistic unit composed of at least a part of speech and a lemma.
        (Gil Francopoulo; http://www.isocat.org/datcat/DC-1415)
	""" ;
      rdfs:label "word" ;
      rdfs:subClassOf <http://purl.org/olia/olia-top.owl#SyntacticCategory> .

<http://purl.org/olia/system.owl#Feature>
      a       owl:Class ;
      rdfs:comment "UnitsOfAnnotation and Relations can be described in a more detailed way by the features that are attached to them, e.g., case, number, or aspect. Features are, however, not subject to further annotations (by means of hasFeature), they are thus disjoint from Relations and UnitsOfAnnotation." ;
      rdfs:subClassOf <http://purl.org/olia/system.owl#LinguisticAnnotation> .

<http://purl.org/olia/penn.owl#NNPS>
      a       owl:Thing .

<http://purl.org/olia/penn.owl#ProperNoun>
      a       owl:Class ;
      rdfs:comment "These are singular or plural proper nouns." ;
      rdfs:subClassOf <http://purl.org/olia/penn.owl#Noun> , <http://purl.org/olia/olia.owl#ProperNoun> .

<http://purl.org/olia/olia.owl#Noun>
      a       owl:Class ;
      rdfs:comment """
	A noun, or noun substantive, is a part of speech (a word or phrase) which can co-occur with 
	(in)definite articles and attributive adjectives, and function as the head of a noun phrase.

	The word \"noun\" derives from the Latin 'nomen' meaning \"name\", and a traditional definition 
	of nouns is that they are all and only those expressions that refer to a person, place, 
	thing, event, substance, quality, idea or an appointment. They serve as the subject or object 
	of a verb, and the object of a preposition.
	(http://en.wikipedia.org/wiki/Noun 19.09.06)
	""" ;
      rdfs:subClassOf <http://purl.org/olia/olia-top.owl#MorphosyntacticCategory> , <http://purl.org/olia/olia-top.owl#Word> .

<http://purl.org/olia/penn.owl#Noun>
      a       owl:Class ;
      rdfs:comment "We inserted this class 'noun' to get a clearer ontology structure. In The Penn Treebank Tag Set there is no class 'noun'." ;
      rdfs:subClassOf <http://purl.org/olia/olia.owl#Noun> , <http://purl.org/olia/penn.owl#Tag> .

owl:Thing
      a       owl:Class .

<http://purl.org/olia/penn.owl#Tag>
      a       owl:Class ;
      rdfs:subClassOf <http://purl.org/olia/system.owl#LinguisticAnnotation> .

<http://purl.org/olia/olia.owl#Plural>
      a       owl:Class ;
      rdfs:comment """
		Plural is a grammatical number, typically referring to more than one of 
		the referent in the real world. In English, nouns, pronouns, and demonstratives 
		inflect for plurality. In many other languages, for example German and the 
		various Romance languages, articles and adjectives also inflect for plurality. 
		(http://en.wikipedia.org/wiki/Plural  17.11.06)
		""" ;
      rdfs:subClassOf <http://purl.org/olia/olia-top.owl#NumberFeature> .

<http://purl.org/olia/olia.owl#ProperNoun>
      a       owl:Class ;
      rdfs:comment """
		Proper nouns (also called proper names) are the names of unique entities. 
		(http://en.wikipedia.org/wiki/Noun 19.09.06)
	""" ;
      rdfs:subClassOf <http://purl.org/olia/olia.owl#Noun> .
