@prefix rdfs:    <http://www.w3.org/2000/01/rdf-schema#> .
@prefix owl:     <http://www.w3.org/2002/07/owl#> .
@prefix xsd:     <http://www.w3.org/2001/XMLSchema#> .
@prefix rdf:     <http://www.w3.org/1999/02/22-rdf-syntax-ns#> .

<http://purl.org/olia/olia.owl#Residual>
      a       owl:Class ;
      rdfs:comment """
      The residual value (R) is assigned to classes of text words which lie outside the 
      traditionally accepted range of grammatical classes, although they occur quite 
      commonly in many texts and very commonly in some. For example: foreign words, 
      or mathematical formulae. It can be argued that these are on the fringes of the 
      grammar or lexicon of the language in which the text is written. Nevertheless, 
      they need to be tagged. (http://www.ilc.cnr.it/EAGLES96/annotate/node16.html#mr 19.09.06)
      
      Although words in the Residual category are on the periphery of the lexicon, they may 
      take some of the grammatical characteristics, e.g., of nouns. Acronyms such as IBM are 
      similar to proper nouns; symbols such as alphabetic characters can vary for singular and 
      plural (e.g. How many Ps are there in `psychopath'?), and are in this respect like common 
      nouns. In some languages (e.g. Portuguese) such symbols also have gender. It is quite 
      reasonable that in some tagging schemes some of these classes of word will be classified 
      under other parts of speech. (The Unclassified category applies to word-like text segments 
      which do not easily fit into any of the foregoing values. For example: incomplete words 
      and pause fillers such as er and erm in transcriptions of speech, or written representations of singing such as dum-de-dum. (http://www.ilc.cnr.it/EAGLES96/annotate/node17.html#recr 19.09.06)""" ;
      rdfs:subClassOf <http://purl.org/olia/olia-top.owl#MorphosyntacticCategory> , <http://purl.org/olia/olia-top.owl#Word> .

owl:Thing
      a       owl:Class .

<http://purl.org/olia/olia-top.owl#LinguisticConcept>
      a       owl:Class ;
      rdfs:comment """The OLiA ontology specifies linguistic concepts on a theoretical basis, as for concepts used in annotations, see system.owl.
There is a great extent of overlap between LinguisticCategories/LinguisticFeatures and Categories/Features as defined in system.owl.""" ;
      rdfs:subClassOf owl:Thing .

<http://purl.org/olia/penn.owl#Tag>
      a       owl:Class ;
      rdfs:subClassOf <http://purl.org/olia/system.owl#LinguisticAnnotation> .

<http://purl.org/olia/penn.owl#Symbol>
      a       owl:Class ;
      rdfs:comment "This tag should be used for mathematical, scientific and technical symbols or expressions that aren't words of English. It should not used for any and all technical expressions. For instance, the names of chemicals, units of measurements (including abbreviations thereof)  and the like should be tagged as nouns." ;
      rdfs:subClassOf <http://purl.org/olia/penn.owl#Tag> , <http://purl.org/olia/olia.owl#Symbol> .

<http://purl.org/olia/olia-top.owl#MorphosyntacticCategory>
      a       owl:Class ;
      rdfs:subClassOf <http://purl.org/olia/olia-top.owl#SyntacticCategory> .

<http://purl.org/olia/system.owl#LinguisticAnnotation>
      a       owl:Class ;
      rdfs:comment "Linguistic annotations pertain to either structural entities (words, tokens, constituents, sentences => UnitOfAnnotation), relations between these (dependency, dominance, coreference, etc. => Relation), or grammatical features attached to these (case, gender, number, agreement, tense, mood, aspect, ... => Feature)." ;
      rdfs:subClassOf owl:Thing .

<http://purl.org/olia/penn.owl#SYM>
      a       owl:Thing .

<http://purl.org/olia/olia-top.owl#SyntacticCategory>
      a       owl:Class ;
      rdfs:subClassOf <http://purl.org/olia/olia-top.owl#LinguisticConcept> .

<http://purl.org/olia/olia.owl#Symbol>
      a       owl:Class ;
      rdfs:comment """
      In morphosyntactic annotation schemes, a symbol is a single graphical sign 
      that occurs in a written text with a conventionalized meaning but that
      does not represent a phoneme (like ordinary characters), an orthogaphic sign (punctuation),
      or a number. (Christian Chiarcos)
      
      Symbols such as alphabetic characters can vary for singular and plural 
      (e.g. How many Ps are there in `psychopath'?), and are in this respect 
      like common nouns. In some languages (e.g. Portuguese) such symbols also have gender. 
      (http://www.ilc.cnr.it/EAGLES96/annotate/node17.html#recr)    
      """ ;
      rdfs:subClassOf <http://purl.org/olia/olia.owl#Residual> .

<http://purl.org/olia/olia-top.owl#Word>
      a       owl:Class ;
      rdfs:comment """
		SyntacticWord is the class of syntactic units occupying the lowest position in 
		a syntactic construction. They are the largest units resistant to insertion of 
		new constituents within their boundaries; or they are the smallest constituents 
		that can be moved within a sentence without making the sentence ungrammatical.
		(http://www.linguistics-ontology.org/gold/2008/SyntacticWord)
		
		Linguistic unit composed of at least a part of speech and a lemma.
        (Gil Francopoulo; http://www.isocat.org/datcat/DC-1415)
	""" ;
      rdfs:label "word" ;
      rdfs:subClassOf <http://purl.org/olia/olia-top.owl#SyntacticCategory> .
