<rdf:RDF
    xmlns:rdf="http://www.w3.org/1999/02/22-rdf-syntax-ns#"
    xmlns:owl="http://www.w3.org/2002/07/owl#"
    xmlns:xsd="http://www.w3.org/2001/XMLSchema#"
    xmlns:rdfs="http://www.w3.org/2000/01/rdf-schema#" > 
  <rdf:Description rdf:about="http://purl.org/olia/olia-top.owl#LinguisticConcept">
    <rdf:type rdf:resource="http://www.w3.org/2002/07/owl#Class"/>
    <rdfs:subClassOf rdf:resource="http://www.w3.org/2002/07/owl#Thing"/>
    <rdfs:comment>The OLiA ontology specifies linguistic concepts on a theoretical basis, as for concepts used in annotations, see system.owl.
There is a great extent of overlap between LinguisticCategories/LinguisticFeatures and Categories/Features as defined in system.owl.</rdfs:comment>
  </rdf:Description>
  <rdf:Description rdf:about="http://purl.org/olia/olia-top.owl#SyntacticCategory">
    <rdfs:subClassOf rdf:resource="http://purl.org/olia/olia-top.owl#LinguisticConcept"/>
    <rdf:type rdf:resource="http://www.w3.org/2002/07/owl#Class"/>
  </rdf:Description>
  <rdf:Description rdf:about="http://purl.org/olia/olia-top.owl#MorphosyntacticCategory">
    <rdf:type rdf:resource="http://www.w3.org/2002/07/owl#Class"/>
    <rdfs:subClassOf rdf:resource="http://purl.org/olia/olia-top.owl#SyntacticCategory"/>
  </rdf:Description>
  <rdf:Description rdf:about="http://purl.org/olia/system.owl#LinguisticAnnotation">
    <rdf:type rdf:resource="http://www.w3.org/2002/07/owl#Class"/>
    <rdfs:subClassOf rdf:resource="http://www.w3.org/2002/07/owl#Thing"/>
    <rdfs:comment>Linguistic annotations pertain to either structural entities (words, tokens, constituents, sentences =&gt; UnitOfAnnotation), relations between these (dependency, dominance, coreference, etc. =&gt; Relation), or grammatical features attached to these (case, gender, number, agreement, tense, mood, aspect, ... =&gt; Feature).</rdfs:comment>
  </rdf:Description>
  <rdf:Description rdf:about="http://purl.org/olia/olia.owl#ing">
    <rdf:type rdf:resource="http://www.w3.org/2002/07/owl#Class"/>
    <rdfs:subClassOf rdf:resource="http://purl.org/olia/olia.owl#Gerund"/>
    <rdfs:subClassOf rdf:resource="http://purl.org/olia/olia.owl#Participle"/>
    <rdfs:comment>English verb forms ending in '-ing' that represent either Gerunds or Participles.</rdfs:comment>
  </rdf:Description>
  <rdf:Description rdf:about="http://purl.org/olia/olia.owl#Gerund">
    <rdfs:comment>
    	property for a non-finite form of a verb other than the infinitive.
    	(http://www.isocat.org/datcat/DC-2243)
    	
	 A gerund is a kind of verbal noun that exists in some languages. In today's English, 
	 gerunds are nouns built from a verb with an '-ing' suffix. They can be used as the 
	 subject of a sentence, an object, or an object of preposition. They can also be used 
	 to complement a subject. Often, gerunds exist side-by-side with nouns that come from 
	 the same root but the gerund and the common noun have different shades of meaning.
	(http://en.wikipedia.org/wiki/Gerund, http://en.wikibooks.org/wiki/English:Gerund 19.09.06)

	The term _gerund_ is ambiguous: with respect  to Latin, in whose grammatical tradition it originates, it refers to a  deverbal noun, and is needed in this function for Polish as well; in  descriptions of some other languages, however, it has been used for an  adverbial participle.  
	The two meanings have nothing in common, except  that the English _ing_-form can translate both. (Ivan A Derzhanski, email 2010/06/09)
	Here, it is assumed that Gerund refers only to deverbal nouns, cf. NominalNonfiniteVerb in the IIIT tagset (http://purl.org/olia/iiit.owl#NominalNonFiniteVerb)
    </rdfs:comment>
    <rdfs:subClassOf rdf:resource="http://purl.org/olia/olia.owl#NonFiniteVerb"/>
    <rdf:type rdf:resource="http://www.w3.org/2002/07/owl#Class"/>
  </rdf:Description>
  <rdf:Description rdf:about="http://purl.org/olia/olia-top.owl#Word">
    <rdf:type rdf:resource="http://www.w3.org/2002/07/owl#Class"/>
    <rdfs:subClassOf rdf:resource="http://purl.org/olia/olia-top.owl#SyntacticCategory"/>
    <rdfs:comment>
		SyntacticWord is the class of syntactic units occupying the lowest position in 
		a syntactic construction. They are the largest units resistant to insertion of 
		new constituents within their boundaries; or they are the smallest constituents 
		that can be moved within a sentence without making the sentence ungrammatical.
		(http://www.linguistics-ontology.org/gold/2008/SyntacticWord)
		
		Linguistic unit composed of at least a part of speech and a lemma.
        (Gil Francopoulo; http://www.isocat.org/datcat/DC-1415)
	</rdfs:comment>
    <rdfs:label>word</rdfs:label>
  </rdf:Description>
  <rdf:Description rdf:about="http://purl.org/olia/penn.owl#Verb">
    <rdf:type rdf:resource="http://www.w3.org/2002/07/owl#Class"/>
    <rdfs:subClassOf rdf:resource="http://purl.org/olia/penn.owl#Tag"/>
    <rdfs:subClassOf rdf:resource="http://purl.org/olia/olia.owl#Verb"/>
    <rdfs:comment>Inserted to structure the tag set.</rdfs:comment>
  </rdf:Description>
  <rdf:Description rdf:about="http://purl.org/olia/olia.owl#NonFiniteVerb">
    <rdf:type rdf:resource="http://www.w3.org/2002/07/owl#Class"/>
    <rdfs:subClassOf rdf:resource="http://purl.org/olia/olia.owl#Verb"/>
    <rdfs:comment>
             Verb forms occurring on their own only in dependent clauses and lacking tense and mood contrasts.
			 (adapted from Crystal 2003; http://www.isocat.org/datcat/DC-1332)
			 
			A non-finite verb is a verb that is not fully inflected for categories that are marked inflectionally in a language, 
			such as the following: Tense, Aspect, Modality, Number,  Person.  
			(http://www.sil.org/linguistics/GlossaryOfLinguisticTerms/WhatIsANonfiniteVerb.htm 19.09.06)
		</rdfs:comment>
  </rdf:Description>
  <rdf:Description rdf:about="http://purl.org/olia/penn.owl#VBG">
    <rdf:type rdf:resource="http://www.w3.org/2002/07/owl#Thing"/>
  </rdf:Description>
  <rdf:Description rdf:about="http://www.w3.org/2002/07/owl#Thing">
    <rdf:type rdf:resource="http://www.w3.org/2002/07/owl#Class"/>
  </rdf:Description>
  <rdf:Description rdf:about="http://purl.org/olia/olia.owl#Verb">
    <rdfs:comment>
		A verb is a part of speech that usually denotes action ("bring", "read"), 
		occurrence ("decompose", "glitter"), or a state of being ("exist", "stand"). 
		Depending on the language, a verb may vary in form according to many factors, 
		possibly including its tense, aspect, mood and voice. It may also agree with 
		the person, gender, and/or number of some of its arguments (subject, object, etc.).
		(http://en.wikipedia.org/wiki/Verb 19.09.06)
	</rdfs:comment>
    <rdfs:subClassOf rdf:resource="http://purl.org/olia/olia-top.owl#MorphosyntacticCategory"/>
    <rdfs:subClassOf rdf:resource="http://purl.org/olia/olia-top.owl#Word"/>
    <rdf:type rdf:resource="http://www.w3.org/2002/07/owl#Class"/>
  </rdf:Description>
  <rdf:Description rdf:about="http://purl.org/olia/penn.owl#Tag">
    <rdfs:subClassOf rdf:resource="http://purl.org/olia/system.owl#LinguisticAnnotation"/>
    <rdf:type rdf:resource="http://www.w3.org/2002/07/owl#Class"/>
  </rdf:Description>
  <rdf:Description rdf:about="http://purl.org/olia/olia.owl#Participle">
    <rdfs:comment>
	A participle is a lexical item, derived from a verb that has some of the characteristics and functions of both verbs and adjectives.
	In English, participles may be used as adjectives, and in non-finite forms of verbs.
	(http://www.sil.org/linguistics/GlossaryOfLinguisticTerms/WhatIsAParticiple.htm 19.09.06)
	</rdfs:comment>
    <rdfs:subClassOf rdf:resource="http://purl.org/olia/olia.owl#NonFiniteVerb"/>
    <rdf:type rdf:resource="http://www.w3.org/2002/07/owl#Class"/>
  </rdf:Description>
  <rdf:Description rdf:about="http://purl.org/olia/penn.owl#GerundOrPresentParticiple">
    <rdf:type rdf:resource="http://www.w3.org/2002/07/owl#Class"/>
    <rdfs:comment>This is a verb in present participle or in gerund.</rdfs:comment>
    <rdfs:subClassOf rdf:resource="http://purl.org/olia/olia.owl#ing"/>
    <rdfs:subClassOf rdf:resource="http://purl.org/olia/penn.owl#Verb"/>
  </rdf:Description>
</rdf:RDF>
